test/kmp_matcher.lean
@@ -1,0 +1,23 @@
+import Std.Tactic.GuardMsgs
+import Std.Data.String.Basic
+
+/-! Tests for Knuth-Morris-Pratt matching algorithm -/
+
+/-- Matcher for pattern "abba" -/
+def m := String.Matcher.ofString "abba"
+
+/-- info: false -/
+#guard_msgs in
+#eval Option.isSome <| m.find? "AbbabbA" -- false
+
+/-- info: true -/
+#guard_msgs in
+#eval Option.isSome <| m.find? "aabbaa" -- true
+
+/-- info: 2 -/
+#guard_msgs in
+#eval Array.size <| m.findAll "abbabba" -- 2
+
+/-- info: 3 -/
+#guard_msgs in
+#eval Array.size <| m.findAll "abbabbabba" -- 3
